theorems/Utils.v
@@ -1,5 +1,3 @@
-Require Import Coq.Strings.String.
-
 Inductive Result (T: Type) (E: Type): Type :=
 	| Ok (value: T)
 	| Err (error: E).
