build.sh
@@ -1,5 +1,3 @@
 pushd theorems
-coq_makefile -f _CoqProject *.v -o Makefile
-make clean
 make
 popd
