fullbuild.sh
@@ -1,0 +1,5 @@
+pushd theorems
+coq_makefile -f _CoqProject *.v -o Makefile
+make clean
+make
+popd
